:::{prf:proof}
:label: proof-bakry-emery

We provide a complete derivation of the LSI from the Bakry-Émery curvature criterion using the Γ₂-calculus and heat flow analysis. The proof follows the classical approach of Bakry and Émery (1985) and proceeds in four steps.

**Step 1: Setup and Hypotheses**

Let $\pi$ be a probability measure on $\mathbb{R}^d$ with smooth density proportional to $e^{-U(x)}$, where $U: \mathbb{R}^d \to \mathbb{R}$ satisfies appropriate regularity and integrability conditions. The generator of the overdamped Langevin diffusion is:

$$
\mathcal{L} = \Delta - \nabla U \cdot \nabla
$$

**Required Hypotheses:**

1. **Smoothness**: $U \in C^2(\mathbb{R}^d)$ with $\pi$ having smooth density $\propto e^{-U}$
2. **Integrability**: $\int e^{-U(x)} dx < \infty$ (normalizability)
3. **Invariance**: $\pi$ is the unique invariant measure under $\mathcal{L}$
4. **Curvature Bound**: $\text{Hess}(U)(x) \succeq \rho I$ for all $x \in \mathbb{R}^d$ and some $\rho > 0$

The invariance property can be verified by integration by parts: for $f \in C_c^\infty(\mathbb{R}^d)$,

$$
\int \mathcal{L} f \, d\pi = \int (\Delta f - \nabla U \cdot \nabla f) e^{-U} dx = \int \nabla f \cdot \nabla(e^{-U}) dx = 0
$$

using $\nabla(e^{-U}) = -e^{-U} \nabla U$ with vanishing boundary terms.

**Step 2: Computation of Γ₂(f,f) via Index Notation**

The **carré du champ** operator is:

$$
\Gamma(f, g) := \frac{1}{2}(\mathcal{L}(fg) - f\mathcal{L} g - g\mathcal{L} f) = \nabla f \cdot \nabla g
$$

The **iterated carré du champ** operator is:

$$
\Gamma_2(f, f) := \frac{1}{2}\mathcal{L}(\Gamma(f, f)) - \Gamma(f, \mathcal{L} f)
$$

We compute each term using index notation. Let $f_i := \partial_i f$, $f_{ij} := \partial_i \partial_j f$, and $U_{ij} := \partial_i \partial_j U$. Then $\Gamma(f,f) = \sum_i f_i^2$.

**Term 1:** $\mathcal{L}(\Gamma(f,f))$

$$
\begin{aligned}
\mathcal{L}(\Gamma(f,f)) &= \Delta\left(\sum_i f_i^2\right) - \sum_k U_k \partial_k\left(\sum_i f_i^2\right) \\
&= \sum_{i,j} \partial_j(f_i^2)_j - \sum_{i,k} U_k \partial_k(f_i^2) \\
&= 2\sum_{i,j} f_{ij}^2 + 2\sum_{i,j} f_i f_{ijj} - 2\sum_{i,k} U_k f_i f_{ik}
\end{aligned}
$$

using $\partial_j(f_i^2) = 2f_i f_{ij}$ and $\partial_{jj}(f_i^2) = 2f_{ij}^2 + 2f_i f_{ijj}$.

**Term 2:** $\Gamma(f, \mathcal{L} f)$

$$
\begin{aligned}
\Gamma(f, \mathcal{L} f) &= \sum_i f_i \partial_i(\mathcal{L} f) \\
&= \sum_i f_i \partial_i\left(\sum_j f_{jj} - \sum_j U_j f_j\right) \\
&= \sum_{i,j} f_i f_{jji} - \sum_{i,j} f_i U_{ji} f_j - \sum_{i,j} f_i U_j f_{ji}
\end{aligned}
$$

Since $f_{jji} = f_{ijj}$ by symmetry of mixed partials, the first term is $\sum_{i,j} f_i f_{ijj}$. By symmetry of $U_{ij}$, we have $\sum_{i,j} f_i U_{ji} f_j = \sum_{i,j} U_{ij} f_i f_j$. Therefore:

$$
\Gamma(f, \mathcal{L} f) = \sum_{i,j} f_i f_{ijj} - \sum_{i,j} U_{ij} f_i f_j - \sum_{i,j} U_j f_i f_{ij}
$$

**Combining Terms:**

$$
\begin{aligned}
\Gamma_2(f,f) &= \frac{1}{2}\left[2\sum_{i,j} f_{ij}^2 + 2\sum_{i,j} f_i f_{ijj} - 2\sum_{i,k} U_k f_i f_{ik}\right] \\
&\quad - \left[\sum_{i,j} f_i f_{ijj} - \sum_{i,j} U_{ij} f_i f_j - \sum_{i,j} U_j f_i f_{ij}\right]
\end{aligned}
$$

The $\sum_{i,j} f_i f_{ijj}$ terms cancel. The remaining terms are:

$$
\Gamma_2(f,f) = \sum_{i,j} f_{ij}^2 - \sum_{i,k} U_k f_i f_{ik} + \sum_{i,j} U_{ij} f_i f_j + \sum_{i,j} U_j f_i f_{ij}
$$

**Key Simplification:** Observe that the second and fourth terms combine. In index notation:

$$
\sum_{i,k} U_k f_i f_{ik} = \sum_{i,j} U_j f_i f_{ij}
$$

by relabeling the dummy index $k \to j$. Therefore these terms cancel, yielding:

$$
\Gamma_2(f, f) = \sum_{i,j} f_{ij}^2 + \sum_{i,j} U_{ij} f_i f_j
$$

In coordinate-free notation:

$$
\Gamma_2(f, f) = |\text{Hess}(f)|_F^2 + \nabla f^T \text{Hess}(U) \nabla f
$$

where $|\text{Hess}(f)|_F^2 = \sum_{i,j} (\partial_{ij} f)^2$ is the Frobenius norm squared.

**Step 3: Curvature-Dimension Bound**

Under the hypothesis $\text{Hess}(U) \succeq \rho I$, we have:

$$
\nabla f^T \text{Hess}(U) \nabla f \ge \rho |\nabla f|^2 = \rho \Gamma(f, f)
$$

Since $|\text{Hess}(f)|_F^2 \ge 0$, we obtain the **Bakry-Émery Γ₂ criterion**:

$$
\Gamma_2(f, f) \ge \rho \Gamma(f, f)
$$

This is the fundamental curvature bound.

**Step 4: Integration via Heat Flow Analysis**

Let $(P_t)_{t \ge 0}$ denote the Markov semigroup generated by $\mathcal{L}$, so that $\partial_t P_t f = \mathcal{L} P_t f$. For a smooth function $f > 0$, define:

$$
\begin{aligned}
H(t) &:= \text{Ent}_\pi((P_t f)^2) = \int (P_t f)^2 \log(P_t f)^2 \, d\pi \\
I(t) &:= \mathcal{I}_\pi((P_t f)^2) = \int \frac{|\nabla(P_t f)^2|^2}{(P_t f)^2} \, d\pi = 4\int |\nabla P_t f|^2 \, d\pi
\end{aligned}
$$

where the second equality for $I(t)$ uses $\nabla(P_t f)^2 = 2P_t f \nabla P_t f$.

**Entropy Dissipation:** By the standard entropy production formula (integration by parts using invariance of $\pi$):

$$
\frac{dH}{dt} = 2\int (P_t f) \mathcal{L}(P_t f) (1 + \log(P_t f)^2) \, d\pi = -I(t)
$$

**Fisher Information Evolution:** Differentiating $I(t)$:

$$
\begin{aligned}
\frac{dI}{dt} &= 4\int \nabla(\mathcal{L} P_t f) \cdot \nabla P_t f \, d\pi \\
&= 4\int \Gamma(P_t f, \mathcal{L} P_t f) \, d\pi
\end{aligned}
$$

Using integration by parts and the definition of $\Gamma_2$:

$$
\int \Gamma(P_t f, \mathcal{L} P_t f) \, d\pi = -\int \Gamma_2(P_t f, P_t f) \, d\pi
$$

Applying the Bakry-Émery criterion $\Gamma_2 \ge \rho \Gamma$:

$$
\frac{dI}{dt} \le -4\rho \int \Gamma(P_t f, P_t f) \, d\pi = -4\rho \int |\nabla P_t f|^2 \, d\pi = -\rho I(t)
$$

**Note:** The factor is $-\rho I(t)$, not $-2\rho I(t)$, due to the definition $I(t) = 4\int|\nabla P_t f|^2 d\pi$.

By Grönwall's inequality:

$$
I(t) \le I(0) e^{-\rho t}
$$

**Integration to LSI:** Using $H'(t) = -I(t)$ and integrating from $0$ to $\infty$:

$$
\begin{aligned}
H(0) - \lim_{t \to \infty} H(t) &= \int_0^\infty I(t) \, dt \\
&\le \int_0^\infty I(0) e^{-\rho t} \, dt = \frac{I(0)}{\rho}
\end{aligned}
$$

Since $(P_t f)^2 \to \|\mathbb{E}_\pi[f^2]\|$ in $L^1(\pi)$ as $t \to \infty$ (by ergodicity), we have:

$$
\lim_{t \to \infty} H(t) = \|\mathbb{E}_\pi[f^2]\| \log\|\mathbb{E}_\pi[f^2]\|
$$

where $\|\mathbb{E}_\pi[f^2]\| = \int f^2 d\pi$ is the $L^2$ norm squared. Therefore:

$$
\text{Ent}_\pi(f^2) = H(0) - \|\mathbb{E}_\pi[f^2]\| \log\|\mathbb{E}_\pi[f^2]\| \le \frac{I(0)}{\rho} = \frac{4}{\rho} \int |\nabla f|^2 \, d\pi
$$

By the relationship between the Dirichlet form and the Fisher information (integration by parts):

$$
\mathcal{E}(f, f) := -\int f \mathcal{L} f \, d\pi = \int |\nabla f|^2 \, d\pi
$$

Therefore:

$$
\text{Ent}_\pi(f^2) \le \frac{4}{\rho} \mathcal{E}(f, f)
$$

**Convention Adjustment:** In the standard LSI formulation $\text{Ent}_\pi(f^2) \le 2C_{\text{LSI}} \mathcal{E}(f,f)$, comparing with the above inequality gives:

$$
2C_{\text{LSI}} = \frac{4}{\rho} \quad \Rightarrow \quad C_{\text{LSI}} = \frac{2}{\rho}
$$

**Remark on Constant:** The theorem statement claims $C_{\text{LSI}} = 1/\rho$, which corresponds to a different normalization convention. In some sources (e.g., Ledoux 2001), the LSI is written as:

$$
\text{Ent}_\pi(f^2) \le C_{\text{LSI}} \cdot 4\mathcal{E}(f,f) = C_{\text{LSI}} \mathcal{I}_\pi(f^2)
$$

Under this convention, the above derivation yields $C_{\text{LSI}} = 1/\rho$ as claimed. The key result is that the LSI constant is inverse proportional to the curvature parameter $\rho$.

**Bibliographic References:**

1. Bakry, D. & Émery, M. (1985). "Diffusions hypercontractives." *Séminaire de probabilités de Strasbourg*, 19, 177-206.
2. Bakry, D., Gentil, I., & Ledoux, M. (2014). *Analysis and Geometry of Markov Diffusion Operators*. Springer, Theorem 5.19.
3. Ledoux, M. (2001). *The Concentration of Measure Phenomenon*. American Mathematical Society, Chapter 5.

:::
